workaround

lexical.dfy
@@ -4,17 +4,7 @@ module Lexical_Order_Strings refines Total_Order {
 
  	type Element = string
 
-	predicate method lte(a: Element, b: Element)
-	{
-		if |a| == 0 && |b| == 0 then true
-		else if |a| == 0       then true
-		else if |b| == 0       then false
-		else if a[0] < b[0]    then true
-		else if a[0] > b[0]    then false
-		else lte(a[1..], b[1..])
-	}
-
-	predicate ltedef(a: Element, b: Element)
+	predicate method ltedef(a: Element, b: Element)
 	{
 		if |a| == 0 && |b| == 0 then true
 		else if |a| == 0       then true
@@ -22,5 +12,18 @@ module Lexical_Order_Strings refines Total_Order {
 		else if a[0] < b[0]    then true
 		else if a[0] > b[0]    then false
 		else ltedef(a[1..], b[1..])
+	}
+
+    lemma ltedef_properties(a: Element, b: Element)
+		ensures ltedef(a, b) || ltedef(b, a); // Total
+		ensures ltedef(a, b) && ltedef(b, a) ==> a == b; // Antisymmetric
+    {
+    }
+
+
+	predicate method lte(a: Element, b: Element)
+	{
+        ltedef_properties(a, b);
+        ltedef(a, b)
 	}
 }
